cleaning for microyalla

yalla/ill_smp.v
@@ -17,26 +17,23 @@ Require ill_cut.
 
 
 (** ** 1. define formulas *)
-Require Export ill.
-
-Lemma pt2ypt : forall A l1 l2, @Permutation_Type A l1 l2 ->
-  @Permutation_Type.Permutation_Type A l1 l2.
-Proof.
-intros A l1 l2 HP ; induction HP ; econstructor ; eassumption.
-Qed.
-
-Lemma ypt2pt : forall A l1 l2, @Permutation_Type.Permutation_Type A l1 l2 ->
-  @Permutation_Type A l1 l2.
-Proof.
-intros A l1 l2 HP ; induction HP ; econstructor ; eassumption.
-Qed.
+Inductive iformula : Set :=
+| ivar  : iformulas.IAtom -> iformula
+| ione  : iformula
+| itens : iformula -> iformula -> iformula
+| ilmap : iformula -> iformula -> iformula
+| itop  : iformula
+| iwith : iformula -> iformula -> iformula
+| izero : iformula
+| iplus : iformula -> iformula -> iformula
+| ioc   : iformula -> iformula.
 
 
 (** ** 2. define embedding into [formulas.formula] *)
 
 Fixpoint ill2ill A :=
 match A with
-| ivar x    => iformulas.ivar (Some x)
+| ivar x    => iformulas.ivar x
 | ione      => iformulas.ione
 | itens A B => iformulas.itens (ill2ill A) (ill2ill B)
 | ilmap A B => iformulas.ilmap (ill2ill A) (ill2ill B)
@@ -81,6 +78,28 @@ Qed.
 
 (** ** 3. define proofs *)
 
+Inductive ill : list iformula -> iformula -> Type :=
+| ax_ir : forall X, ill (ivar X :: nil) (ivar X)
+| ex_ir : forall l1 l2 A, ill l1 A -> Permutation_Type l1 l2 -> ill l2 A
+| one_irr : ill nil ione
+| one_ilr : forall l A, ill l A -> ill (ione :: l) A
+| tens_irr : forall A B l1 l2, ill l1 A -> ill l2 B -> ill (l1 ++ l2) (itens A B)
+| tens_ilr : forall A B l C, ill (A :: B :: l) C -> ill (itens A B :: l) C
+| lmap_irr : forall A B l, ill (A :: l) B -> ill l (ilmap A B)
+| lmap_ilr : forall A B l1 l2 C, ill l1 A -> ill (B :: l2) C -> ill (ilmap A B :: l1 ++ l2) C
+| top_irr : forall l, ill l itop
+| with_irr : forall A B l, ill l A -> ill l B -> ill l (iwith A B)
+| with_ilr1 : forall A B l C, ill (A :: l) C -> ill (iwith A B :: l) C
+| with_ilr2 : forall A B l C, ill (A :: l) C -> ill (iwith B A :: l) C
+| zero_ilr : forall l C, ill (izero :: l) C
+| plus_irr1 : forall A B l, ill l A -> ill l (iplus A B)
+| plus_irr2 : forall A B l, ill l A -> ill l (iplus B A)
+| plus_ilr : forall A B l C, ill (A :: l) C -> ill (B :: l) C -> ill (iplus A B :: l) C
+| oc_irr : forall A l, ill (List.map ioc l) A -> ill (List.map ioc l) (ioc A)
+| de_ilr : forall A l C, ill (A :: l) C -> ill (ioc A :: l) C
+| wk_ilr : forall A l C, ill l C -> ill (ioc A :: l) C
+| co_ilr : forall A l C, ill (ioc A :: ioc A :: l) C -> ill (ioc A :: l) C.
+
 Instance ill_perm {C} : Proper ((@Permutation_Type _) ==> Basics.arrow) (fun l => ill l C).
 Proof.
 intros l1 l2 HP pi.
@@ -99,8 +118,7 @@ Lemma ill2illfrag : forall l A, ill l A -> ill_ll (map ill2ill l) (ill2ill A).
 Proof with try eassumption ; try reflexivity. 
 intros l A pi.
 induction pi ; rewrite <- (app_nil_l _) ; try (now constructor) ; try rewrite map_app.
-- apply pt2ypt in p.
-  eapply ill_def.ex_ir...
+- eapply ill_def.ex_ir...
   apply Permutation_Type_map...
 - rewrite app_nil_l ; constructor...
 - eapply ill_def.ex_ir.
@@ -125,13 +143,11 @@ revert l Heql0 A HeqA0 ; induction pi ; intros l' Heql0 A' HeqA0 ; subst ;
 - destruct A' ; inversion HeqA0.
   destruct l' ; inversion Heql0 ; destruct l' ; inversion Heql0.
   destruct i0 ; inversion H3 ; subst.
-  inversion H4 ; subst.
   apply ax_ir.
 - simpl in p.
   apply Permutation_Type_map_inv in p.
   destruct p as [l'' Heq HP].
   apply Permutation_Type_sym in HP.
-  apply ypt2pt in HP.
   eapply ex_ir...
   apply IHpi...
 - decomp_map_Type Heql0 ; subst.
@@ -141,7 +157,6 @@ revert l Heql0 A HeqA0 ; induction pi ; intros l' Heql0 A' HeqA0 ; subst ;
   eapply ex_ir ;
     [ apply IHpi ; try reflexivity ;
       rewrite <- ill2ill_map_ioc ; rewrite <- ? map_app | ]...
-  apply ypt2pt.
   apply Permutation_Type_app_head.
   apply Permutation_Type_app_tail.
   symmetry in HP ; apply Permutation_Type_map...
@@ -154,7 +169,7 @@ revert l Heql0 A HeqA0 ; induction pi ; intros l' Heql0 A' HeqA0 ; subst ;
   + apply one_ilr.
     apply IHpi...
     rewrite <- ? map_app...
-  + apply ypt2pt ; perm_Type_solve.
+  + perm_Type_solve.
 - decomp_map_Type Heql0 ; subst.
   destruct x ; inversion Heql0 ; subst.
   eapply ex_ir.
@@ -162,10 +177,12 @@ revert l Heql0 A HeqA0 ; induction pi ; intros l' Heql0 A' HeqA0 ; subst ;
     eapply (ex_ir _ (x1 :: x2 :: l0 ++ l4)).
     * apply (IHpi (l0 ++ x1 :: x2 :: l4))...
       simpl ; rewrite map_app...
-    * apply ypt2pt ; perm_Type_solve.
-  + apply ypt2pt ; perm_Type_solve.
+    * perm_Type_solve.
+  + perm_Type_solve.
 - decomp_map_Type Heql0 ; subst.
   destruct x ; inversion Heql0.
+- decomp_map_Type Heql0 ; subst.
+  destruct x; inversion Heql2.
 - decomp_map_Type Heql0 ; subst.
   destruct x ; inversion Heql3 ; subst.
   eapply ex_ir.
@@ -174,8 +191,10 @@ revert l Heql0 A HeqA0 ; induction pi ; intros l' Heql0 A' HeqA0 ; subst ;
     * eapply (ex_ir (l3 ++ x2 :: l7) (x2 :: l3 ++ l7)).
       -- apply IHpi2...
          simpl ; rewrite map_app...
-      -- apply ypt2pt ; perm_Type_solve.
-  + apply ypt2pt ; perm_Type_solve.
+      -- perm_Type_solve.
+  + perm_Type_solve.
+- decomp_map_Type Heql0 ; subst.
+  destruct x; inversion Heql0.
 - decomp_map_Type Heql0 ; subst.
   destruct x ; inversion Heql0 ; subst.
   eapply ex_ir.
@@ -183,8 +202,8 @@ revert l Heql0 A HeqA0 ; induction pi ; intros l' Heql0 A' HeqA0 ; subst ;
     eapply (ex_ir _ (x1 :: l0 ++ l4)).
     * apply (IHpi (l0 ++ x1 :: l4))...
       simpl ; rewrite map_app...
-    * apply ypt2pt ; perm_Type_solve.
-  + apply ypt2pt ; perm_Type_solve.
+    * perm_Type_solve.
+  + perm_Type_solve.
 - decomp_map_Type Heql0 ; subst.
   destruct x ; inversion Heql0 ; subst.
   eapply ex_ir.
@@ -192,13 +211,13 @@ revert l Heql0 A HeqA0 ; induction pi ; intros l' Heql0 A' HeqA0 ; subst ;
     eapply (ex_ir _ (x2 :: l0 ++ l4)).
     * apply (IHpi (l0 ++ x2 :: l4))...
       simpl ; rewrite map_app...
-    * apply ypt2pt ; perm_Type_solve.
-  + apply ypt2pt ; perm_Type_solve.
+    * perm_Type_solve.
+  + perm_Type_solve.
 - decomp_map_Type Heql0 ; subst.
   destruct x ; inversion Heql0 ; subst.
   eapply ex_ir.
   + eapply (zero_ilr (l0 ++ l4)).
-  + apply ypt2pt ; perm_Type_solve.
+  + perm_Type_solve.
 - decomp_map_Type Heql0 ; subst.
   destruct x ; inversion Heql0 ; subst.
   eapply ex_ir.
@@ -206,12 +225,12 @@ revert l Heql0 A HeqA0 ; induction pi ; intros l' Heql0 A' HeqA0 ; subst ;
     * eapply (ex_ir _ (x1 :: l0 ++ l4)).
       -- apply (IHpi1 (l0 ++ x1 :: l4))...
          simpl ; rewrite map_app...
-      -- apply ypt2pt ; perm_Type_solve.
+      -- perm_Type_solve.
     * eapply (ex_ir _ (x2 :: l0 ++ l4)).
       -- apply (IHpi2 (l0 ++ x2 :: l4))...
          simpl ; rewrite map_app...
-      -- apply ypt2pt ; perm_Type_solve.
-  + apply ypt2pt ; perm_Type_solve.
+      -- perm_Type_solve.
+  + perm_Type_solve.
 - destruct A' ; inversion HeqA0 ; subst.
   apply ill2ill_map_ioc_inv in Heql0.
   destruct Heql0 as (l'' & Heq1 & Heq2) ; subst.
@@ -225,15 +244,15 @@ revert l Heql0 A HeqA0 ; induction pi ; intros l' Heql0 A' HeqA0 ; subst ;
     eapply (ex_ir _ (x :: l0 ++ l4)).
     * apply (IHpi (l0 ++ x :: l4))...
       simpl ; rewrite map_app...
-    * apply ypt2pt ; perm_Type_solve.
-  + apply ypt2pt ; perm_Type_solve.
+    * perm_Type_solve.
+  + perm_Type_solve.
 - decomp_map_Type Heql0 ; subst.
   destruct x ; inversion Heql0 ; subst.
   eapply ex_ir.
   + apply wk_ilr.
     apply (IHpi (l0 ++ l4))...
     simpl ; rewrite map_app...
-  + apply ypt2pt ; perm_Type_solve.
+  + perm_Type_solve.
 - decomp_map_Type Heql0 ; subst.
   destruct x ; inversion Heql0 ; subst.
   eapply ex_ir.
@@ -241,8 +260,8 @@ revert l Heql0 A HeqA0 ; induction pi ; intros l' Heql0 A' HeqA0 ; subst ;
     eapply (ex_ir _ (ioc x :: ioc x :: l0 ++ l4)).
     * apply (IHpi (l0 ++ ioc x :: ioc x :: l4))...
       simpl ; rewrite map_app...
-    * apply ypt2pt ; perm_Type_solve.
-  + apply ypt2pt ; perm_Type_solve.
+    * perm_Type_solve.
+  + perm_Type_solve.
 - destruct a.
 Qed.
 
@@ -272,5 +291,4 @@ apply ill2illfrag in pi2.
 eapply ill_cut.cut_ir_axfree...
 intros a ; destruct a.
 Qed.
-
 
